Weidenbach_Book/Watched_Literals_Watch_List_Enumeration.thy
@@ -12,12 +12,109 @@ fun propagate_unit_and_add_wl :: \<open>'v literal \<Rightarrow> 'v twl_st_wl \<
   \<open>propagate_unit_and_add_wl K (M, N, D, NE, UE, Q, W) =
       (Propagated (-K) 0 # M, N, None, add_mset {#-K#} NE, UE, {#K#}, W)\<close>
 
-definition negate_mode_bj_unit_wl   :: \<open>'v twl_st_l \<Rightarrow> 'v twl_st_l nres\<close> where
+definition negate_mode_bj_unit_wl   :: \<open>'v twl_st_wl \<Rightarrow> 'v twl_st_wl nres\<close> where
 \<open>negate_mode_bj_unit_wl = (\<lambda>S. do {
-    (S, K) \<leftarrow> find_decomp_target 1 S;
-    RETURN (propagate_unit_and_add_l K S)
+    (S, K) \<leftarrow> find_decomp_target_wl 1 S;
+    ASSERT(K \<in># all_lits_of_mm (clause `# twl_clause_of `# ran_mf (get_clauses_wl S) +
+           get_unit_init_clss_wl S));
+    RETURN (propagate_unit_and_add_wl K S)
   })\<close>
 
+(* TODO Move *)
+lemma in_all_lits_of_mm_uminusD: \<open>x2 \<in># all_lits_of_mm N \<Longrightarrow> -x2 \<in># all_lits_of_mm N\<close>
+  by (auto simp: all_lits_of_mm_def)
+(* End Move *)
+
+lemma find_decomp_target_wl_find_decomp_target_l:
+  assumes
+    SS': \<open>(S, S') \<in> state_wl_l None\<close> and
+    inv: \<open>negate_mode_bj_unit_l_inv S'\<close> and
+    corr: \<open>correct_watching S\<close> and
+    [simp]: \<open>a = a'\<close>
+  shows \<open>find_decomp_target_wl a S \<le>
+     \<Down> {((S, K), (S', K')). (S, S') \<in> {(S, S'). (S, S') \<in> state_wl_l None \<and> correct_watching S} \<and>
+        (K , K') \<in> Id \<and> K \<in># all_lits_of_mm (clause `# twl_clause_of `# ran_mf (get_clauses_wl S) +
+          get_unit_init_clss_wl S)}
+    (find_decomp_target a' S')\<close>
+    (is \<open>_ \<le> \<Down> ?negate _\<close>)
+proof -
+  let ?y0 = \<open>\<lambda>S S'. (\<lambda>(M, Oth). (get_trail_wl S, Oth)) S'\<close>
+  have K: \<open>K \<in># all_lits_of_mm (clause `# twl_clause_of `# ran_mf (get_clauses_wl S) +
+          get_unit_init_clss_wl S)\<close>
+    if K: \<open>K \<in> lits_of_l (get_trail_wl S)\<close>
+    for K
+  proof -
+    obtain b S'' where
+      S'_S'': \<open>(S', S'') \<in> twl_st_l b\<close> and
+      struct: \<open>twl_struct_invs S''\<close>
+      using inv unfolding negate_mode_bj_unit_l_inv_def by blast
+    then have no_alien: \<open>cdcl\<^sub>W_restart_mset.cdcl\<^sub>W_all_struct_inv (state\<^sub>W_of S'')\<close>
+      using struct unfolding twl_struct_invs_def by fast
+    then have no_alien: \<open>cdcl\<^sub>W_restart_mset.no_strange_atm (state\<^sub>W_of S'')\<close>
+      unfolding cdcl\<^sub>W_restart_mset.cdcl\<^sub>W_all_struct_inv_def by fast
+    moreover have \<open>atms_of_mm (get_all_init_clss S'') =
+          atms_of_mm (mset `# (ran_mf (get_clauses_wl S)) + get_unit_init_clss_wl S)\<close>
+      apply (subst all_clss_lf_ran_m[symmetric])
+      using no_alien 
+      using S'_S'' SS' K unfolding cdcl\<^sub>W_restart_mset.no_strange_atm_def
+      by (cases S; cases S'; cases b)
+        (auto simp: mset_take_mset_drop_mset' cdcl\<^sub>W_restart_mset_state
+        in_all_lits_of_mm_ain_atms_of_iff twl_st_l_def state_wl_l_def)
+    ultimately show ?thesis
+      using S'_S'' SS' K unfolding cdcl\<^sub>W_restart_mset.no_strange_atm_def
+      by (auto simp: twl_st_l twl_st mset_take_mset_drop_mset'
+        in_all_lits_of_mm_ain_atms_of_iff)
+  qed
+  show ?thesis
+    using SS' corr
+    unfolding find_decomp_target_wl_def find_decomp_target_def apply -
+    apply (rule RES_refine)
+    apply (rule_tac x=\<open>(?y0 (fst s) S', snd s)\<close> in bexI)
+    subgoal
+      using K
+      by (cases S; cases S')
+        (auto simp: state_wl_l_def correct_watching.simps clause_to_update_def
+        mset_take_mset_drop_mset')
+    subgoal
+      by (cases S; cases S')
+        (auto simp: state_wl_l_def correct_watching.simps clause_to_update_def)
+    done
+qed
+
+lemma negate_mode_bj_unit_l:
+  fixes S :: \<open>'v twl_st_wl\<close> and S' :: \<open>'v twl_st_l\<close>
+  assumes \<open>count_decided (get_trail_wl S) = 1\<close> and
+    SS': \<open>(S, S') \<in> state_wl_l None\<close> and
+    confl: \<open>get_conflict_wl S = None\<close> and
+    corr: \<open>correct_watching S\<close>
+  shows
+    \<open>negate_mode_bj_unit_wl S \<le> \<Down>{(S, S'). (S, S') \<in> state_wl_l None \<and> correct_watching S}
+       (negate_mode_bj_unit_l S')\<close>
+       (is \<open>_ \<le> \<Down> ?R _\<close>)
+proof -
+  have 2: \<open>(propagate_unit_and_add_wl x2a x1a, propagate_unit_and_add_l x2 x1)
+        \<in> {(S, S''). (S, S'') \<in> state_wl_l None \<and> correct_watching S}\<close>
+    if 
+      \<open>(x, x') \<in> {((S, K), (S', K')). (S, S') \<in> {(S, S'). (S, S') \<in> state_wl_l None \<and> correct_watching S} \<and>
+        (K , K') \<in> Id \<and> K \<in># all_lits_of_mm (clause `# twl_clause_of `# ran_mf (get_clauses_wl S) +
+          get_unit_init_clss_wl S)}\<close> and
+      \<open>x' = (x1, x2)\<close> and
+      \<open>x = (x1a, x2a)\<close>
+    for x2a x1a x2 x1 and x :: \<open>'v twl_st_wl \<times> 'v literal\<close> and x' :: \<open>'v twl_st_l \<times> 'v literal\<close>
+  proof -
+    show ?thesis
+      using that
+      by (cases x1a; cases x1)
+        (auto simp: state_wl_l_def correct_watching.simps clause_to_update_def
+          all_lits_of_mm_add_mset
+          all_lits_of_m_add_mset all_lits_of_mm_union mset_take_mset_drop_mset'
+          dest: in_all_lits_of_mm_uminusD)
+  qed
+
+  show ?thesis
+    using SS' corr unfolding negate_mode_bj_unit_wl_def negate_mode_bj_unit_l_def
+    by (refine_rcg find_decomp_target_wl_find_decomp_target_l 2) auto
+qed
 
 fun propagate_nonunit_and_add_wl
   :: \<open>'v literal \<Rightarrow> 'v clause_l \<Rightarrow> nat \<Rightarrow> 'v twl_st_wl \<Rightarrow> 'v twl_st_wl nres\<close>
@@ -39,4 +136,23 @@ definition negate_mode_bj_nonunit_wl :: \<open>'v twl_st_wl \<Rightarrow> 'v twl
     propagate_nonunit_and_add_wl K C i S
   })\<close>
 
+
+lemma negate_mode_bj_nonunit_l:
+  fixes S :: \<open>'v twl_st_wl\<close> and S' :: \<open>'v twl_st_l\<close>
+  assumes \<open>count_decided (get_trail_wl S) = 1\<close> and
+    SS': \<open>(S, S') \<in> state_wl_l None\<close> and
+    confl: \<open>get_conflict_wl S = None\<close> and
+    corr: \<open>correct_watching S\<close>
+  shows
+    \<open>negate_mode_bj_nonunit_wl S \<le> \<Down>{(S, S''). (S, S'') \<in> state_wl_l None \<and> correct_watching S}
+       (negate_mode_bj_nonunit_l S')\<close>
+proof -
+
+  show ?thesis
+    using corr SS'
+    unfolding negate_mode_bj_nonunit_wl_def negate_mode_bj_nonunit_l_def
+    apply (refine_rcg find_decomp_target_wl_find_decomp_target_l)
+    subgoal 
+      unfolding negate_mode_bj_nonunit_l_inv_def negate_mode_bj_unit_l_inv_def
+    using SS' by (auto simp: )
 end
